feat: `Nat.sub` in cutsat (#7503)
This PR implements support for `Nat.sub` in cutsat

src/Init/Data/Int/Linear.lean
@@ -1658,6 +1658,28 @@ theorem emod_le (x y : Int) (n : Int) : emod_le_cert y n → x % y + n ≤ 0 := 
 theorem natCast_nonneg (x : Nat) : (-1:Int) * NatCast.natCast x ≤ 0 := by
   simp
 
+abbrev natCast_sub_def (x y : Nat) : Int :=
+  if (NatCast.natCast y : Int) + (-1)*NatCast.natCast x ≤ 0 then (NatCast.natCast x : Int) + -1*NatCast.natCast y else (0 : Int)
+
+theorem natCast_sub (x y : Nat) (z : Int)
+    : natCast_sub_def x y = z → (NatCast.natCast (x - y) : Int) = z := by
+  intro; subst z
+  show (↑(x - y) : Int) = if (↑y : Int) + (-1)*↑x ≤ 0 then ↑x + (-1)*↑y else 0
+  rw [Int.neg_mul, ← Int.sub_eq_add_neg, Int.one_mul]
+  rw [Int.neg_mul, ← Int.sub_eq_add_neg, Int.one_mul]
+  split
+  next h =>
+    replace h := Int.le_of_sub_nonpos h
+    rw [Int.ofNat_le] at h
+    rw [Int.ofNat_sub h]
+  next h =>
+    have : ¬ (↑y : Int) ≤ ↑x := by
+      intro h
+      replace h := Int.sub_nonpos_of_le h
+      contradiction
+    rw [Int.ofNat_le] at this
+    rw [Lean.Omega.Int.ofNat_sub_eq_zero this]
+
 private theorem dvd_le_tight' {d p b₁ b₂ : Int} (hd : d > 0) (h₁ : d ∣ p + b₁) (h₂ : p + b₂ ≤ 0)
     : p + (b₁ - d*((b₁-b₂) / d)) ≤ 0 := by
   have ⟨k, h⟩ := h₁
